Added proofs for pointwise PCM building

ulib/experimental/Steel.PCM.ArrayStruct.fst
@@ -13,6 +13,7 @@
    See the License for the specific language governing permissions and
    limitations under the License.
 *)
+
 module Steel.PCM.ArrayStruct
 module U32 = FStar.UInt32
 module Univ = FStar.Universe
@@ -33,38 +34,33 @@ type field_id = string
 
 /// The descriptor contains all the information necessary to derive the type of the values
 /// corresponding to an arraystruct.
-noeq type array_struct_descriptor : Type u#(a+1) =
-  | DBase:
-    a: Type u#a ->
-    array_struct_descriptor
-  | DArray:
-    cell_descriptor:array_struct_descriptor u#a ->
-    len:usize ->
-    array_struct_descriptor
-  | DStruct:
-    field_descriptors: (field_id ^-> array_struct_descriptor u#a) ->
-    array_struct_descriptor
-  // Missing: untagged unions (not must have)
+noeq
+type array_struct_descriptor : Type u#(a + 1) =
+  | DBase : a: Type u#a -> array_struct_descriptor
+  | DArray : cell_descriptor: array_struct_descriptor u#a -> len: usize -> array_struct_descriptor
+  | DStruct : field_descriptors: (field_id ^-> array_struct_descriptor u#a)
+    -> array_struct_descriptor
 
-unfold let struct_field_type'
-  (field_descriptors: (field_id ^-> array_struct_descriptor u#a))
-  (array_struct_type: (descriptor: array_struct_descriptor u#a{
-    descriptor << field_descriptors
-  }) -> Tot (Type u#a))
-  (field: field_id)
-  : Tot (Type u#a) =
+// Missing: untagged unions (not must have)
+unfold
+let struct_field_type'
+      (field_descriptors: (field_id ^-> array_struct_descriptor u#a))
+      (array_struct_type:
+          (descriptor: array_struct_descriptor u#a {descriptor << field_descriptors}
+              -> Tot (Type u#a)))
+      (field: field_id)
+    : Tot (Type u#a) =
   let descr = field_descriptors field in
   FStar.WellFounded.axiom1 field_descriptors field;
   array_struct_type descr
 
-let array_type (cell_type: Type u#a) (len: usize) : Type u#a =
-  Seq.lseq cell_type (v_usize len)
+let array_type (cell_type: Type u#a) (len: usize) : Type u#a = Seq.lseq cell_type (v_usize len)
 
-let struct_type (field_typs: field_id -> Type u#a) : Type u#a =
-  DepMap.t field_id field_typs
+let struct_type (field_typs: (field_id -> Type u#a)) : Type u#a = DepMap.t field_id field_typs
 
 /// This functions achives the descriptor -> Type correspondence
-let rec array_struct_type (descriptor: array_struct_descriptor u#a) : Tot (Type u#a) (decreases descriptor) =
+let rec array_struct_type (descriptor: array_struct_descriptor u#a)
+    : Tot (Type u#a) (decreases descriptor) =
   match descriptor with
   | DBase a -> a
   | DArray descriptor' len ->
@@ -73,140 +69,222 @@ let rec array_struct_type (descriptor: array_struct_descriptor u#a) : Tot (Type 
   | DStruct field_descriptors ->
     let typs' = struct_field_type' field_descriptors array_struct_type in
     struct_type typs'
+unfold
+let struct_field_type
+      (field_descriptors: (field_id ^-> (array_struct_descriptor u#a)))
+      (field: field_id)
+    : Tot (Type u#a) = struct_field_type' field_descriptors array_struct_type field
+noeq
+type array_struct : Type u#(a + 1) =
+  | ArrayStruct : 
+      descriptor: array_struct_descriptor u#a ->
+      pcm: unitless_pcm (array_struct_type descriptor) ->
+      value: array_struct_type descriptor
+    -> array_struct
 
-unfold let struct_field_type
-  (field_descriptors: (field_id ^-> (array_struct_descriptor u#a)))
-  (field: field_id)
-  : Tot (Type u#a) =
-  struct_field_type' field_descriptors array_struct_type field
-
-noeq type array_struct : Type u#(a+1) =
-  | ArrayStruct:
-    descriptor: array_struct_descriptor u#a ->
-    pcm: unitless_pcm (array_struct_type descriptor) ->
-    value: array_struct_type descriptor ->
-    array_struct
-
-let struct_field_type_unroll_lemma
-  (field_descriptors : (field_id ^-> array_struct_descriptor u#a))
-    : Lemma (
-      DependentMap.t u#a field_id (struct_field_type u#a field_descriptors) ==
-      array_struct_type u#a (DStruct u#a field_descriptors)
-     )
-  =
+let struct_field_type_unroll_lemma (field_descriptors: (field_id ^-> array_struct_descriptor u#a))
+    : Lemma
+    (DependentMap.t u#a field_id (struct_field_type u#a field_descriptors) ==
+      array_struct_type u#a (DStruct u#a field_descriptors)) =
   let open FStar.Tactics in
-  assert (
-    DependentMap.t field_id (struct_field_type field_descriptors) ==
-    array_struct_type (DStruct field_descriptors)
-  ) by begin
-    compute ()
-  end
+  FStar.Tactics.Effect.assert_by_tactic (DependentMap.t field_id
+        (struct_field_type field_descriptors) ==
+      array_struct_type (DStruct field_descriptors))
+    (fun _ ->
+        ();
+        compute ())
 
 /// Composability is then based on the composability of the nested PCM.
-let composable_array_struct : symrel u#(a+1) (array_struct u#a) = fun (s0 s1: array_struct u#a) ->
-  s0.descriptor == s1.descriptor /\ s0.pcm == s1.pcm /\
-  s0.pcm.unitless_p.unitless_composable s0.value s1.value
+let composable_array_struct:symrel u#(a + 1) (array_struct u#a) =
+  fun (s0: array_struct u#a) (s1: array_struct u#a) ->
+    s0.descriptor == s1.descriptor /\ s0.pcm == s1.pcm /\
+    s0.pcm.unitless_p.unitless_composable s0.value s1.value
 
 let compose_array_struct
-  (s0: array_struct u#a)
-  (s1: array_struct u#a{s0 `composable_array_struct` s1})
-    : array_struct u#a
-  =
+      (s0: array_struct u#a)
+      (s1: array_struct u#a {s0 `composable_array_struct` s1})
+    : array_struct u#a =
   let new_val = s0.pcm.unitless_p.unitless_op s0.value s1.value in
   ArrayStruct s0.descriptor s0.pcm new_val
 
 #set-options "--print_universes --print_implicits"
 
-let array_struct_unitless_pcm' : unitless_pcm' u#(a+1) (array_struct u#a) = {
-  unitless_composable = composable_array_struct u#a;
-  unitless_op = compose_array_struct u#a;
-}
+let array_struct_unitless_pcm':unitless_pcm' u#(a + 1) (array_struct u#a) =
+  { unitless_composable = composable_array_struct u#a; unitless_op = compose_array_struct u#a }
 
-let array_struct_unitless_pcm : unitless_pcm u#(a+1) (array_struct u#a) = {
-  unitless_p = array_struct_unitless_pcm' u#a;
-  unitless_comm = (fun s0 s1  -> s0.pcm.unitless_comm s0.value s1.value);
-  unitless_assoc = (fun s0 s1 s2 -> s0.pcm.unitless_assoc s0.value s1.value s2.value);
-  unitless_assoc_r = (fun s0 s1 s2 -> s0.pcm.unitless_assoc_r s0.value s1.value s2.value);
-}
+let array_struct_unitless_pcm:unitless_pcm u#(a + 1) (array_struct u#a) =
+  {
+    unitless_p = array_struct_unitless_pcm' u#a;
+    unitless_comm = (fun s0 s1 -> s0.pcm.unitless_comm s0.value s1.value);
+    unitless_assoc = (fun s0 s1 s2 -> s0.pcm.unitless_assoc s0.value s1.value s2.value);
+    unitless_assoc_r = (fun s0 s1 s2 -> s0.pcm.unitless_assoc_r s0.value s1.value s2.value)
+  }
 
-let array_struct_pcm : pcm u#(a+1) (option u#(a+1) (array_struct u#a)) =
+let array_struct_pcm:pcm u#(a + 1) (option u#(a + 1) (array_struct u#a)) =
   to_full_pcm_with_unit array_struct_unitless_pcm
 
 ////////////////////////////////////////////////////////////////////
 // PCM builders
 ////////////////////////////////////////////////////////////////////
 
-let pointwise_array_pcm
-  (cell_type: Type u#a)
-  (len: usize)
-  (base_pcm: unitless_pcm cell_type)
-    : unitless_pcm (array_type cell_type len)
-  =
-  let composable_cell (x y: array_type cell_type len) (i:nat{i < v_usize len}) : prop =
+let pointwise_array_pcm (cell_type: Type u#a) (len: usize) (base_pcm: unitless_pcm cell_type)
+    : unitless_pcm (array_type cell_type len) =
+  let composable_cell (x y: array_type cell_type len) (i: nat{i < v_usize len}) : prop =
     let xi = Seq.index x i in
     let yi = Seq.index y i in
     base_pcm.unitless_p.unitless_composable xi yi
   in
-  let composable : symrel (array_type cell_type len) =
-    fun x y -> forall (i:nat{i < v_usize len}). composable_cell x y i
+  let composable:symrel (array_type cell_type len) =
+    fun x y -> forall (i: nat{i < v_usize len}). composable_cell x y i
   in
-  let compose
-    (x: array_type cell_type len)
-    (y: array_type cell_type len{composable x y})
-      : array_type cell_type len
-    =
-    Seq.init (v_usize len) (fun i ->
-      let xi = Seq.index x i in
-      let yi = Seq.index y i in
-      base_pcm.unitless_p.unitless_op xi yi
-    )
+  let compose (x: array_type cell_type len) (y: array_type cell_type len {composable x y})
+      : array_type cell_type len =
+    Seq.init (v_usize len)
+      (fun i ->
+          let xi = Seq.index x i in
+          let yi = Seq.index y i in
+          base_pcm.unitless_p.unitless_op xi yi)
   in
-  let pcm' : unitless_pcm' (array_type cell_type len) = {
-    unitless_composable = composable;
-    unitless_op = compose;
-  } in
+  let pcm':unitless_pcm' (array_type cell_type len) =
+    { unitless_composable = composable; unitless_op = compose }
+  in
   {
     unitless_p = pcm';
-    (* The proofs here should simply follow by generalization for all indexes *)
-    unitless_comm = (fun x y -> admit());
-    unitless_assoc = (fun _ _ _ -> admit());
-    unitless_assoc_r = (fun _ _ _ -> admit());
+    unitless_comm
+    =
+    (fun x y ->
+        let xy = pcm'.unitless_op x y in
+        let yx = pcm'.unitless_op y x in
+        let aux (i: nat{i < v_usize len}) : Lemma (Seq.index xy i == Seq.index yx i) =
+          base_pcm.unitless_comm (Seq.index x i) (Seq.index y i)
+        in
+        Classical.forall_intro aux;
+        assert (xy `Seq.equal` yx));
+    unitless_assoc
+    =
+    (fun x y z ->
+        let x_yz = pcm'.unitless_op x (pcm'.unitless_op y z) in
+        let aux (i: nat{i < v_usize len})
+            : Lemma
+            (let xi = Seq.index x i in
+              let yi = Seq.index y i in
+              let zi = Seq.index z i in
+              base_pcm.unitless_p.unitless_composable xi yi /\
+              base_pcm.unitless_p.unitless_composable (base_pcm.unitless_p.unitless_op xi yi) zi /\
+              base_pcm.unitless_p.unitless_op xi (base_pcm.unitless_p.unitless_op yi zi) ==
+              base_pcm.unitless_p.unitless_op (base_pcm.unitless_p.unitless_op xi yi) zi) =
+          let xi = Seq.index x i in
+          let yi = Seq.index y i in
+          let zi = Seq.index z i in
+          base_pcm.unitless_assoc xi yi zi
+        in
+        Classical.forall_intro aux;
+        let xy_z = pcm'.unitless_op (pcm'.unitless_op x y) z in
+        assert (x_yz `Seq.equal` xy_z));
+    unitless_assoc_r
+    =
+    (fun x y z ->
+        let xy_z = pcm'.unitless_op (pcm'.unitless_op x y) z in
+        let aux (i: nat{i < v_usize len})
+            : Lemma
+            (let xi = Seq.index x i in
+              let yi = Seq.index y i in
+              let zi = Seq.index z i in
+              base_pcm.unitless_p.unitless_composable yi zi /\
+              base_pcm.unitless_p.unitless_composable xi (base_pcm.unitless_p.unitless_op yi zi) /\
+              base_pcm.unitless_p.unitless_op (base_pcm.unitless_p.unitless_op xi yi) zi ==
+              base_pcm.unitless_p.unitless_op xi (base_pcm.unitless_p.unitless_op yi zi)) =
+          let xi = Seq.index x i in
+          let yi = Seq.index y i in
+          let zi = Seq.index z i in
+          base_pcm.unitless_assoc_r xi yi zi
+        in
+        Classical.forall_intro aux;
+        let x_yz = pcm'.unitless_op x (pcm'.unitless_op y z) in
+        assert (x_yz `Seq.equal` xy_z))
   }
 
 let pointwise_struct_pcm
-  (field_types: field_id -> Type u#a)
-  (base_pcms: (field:field_id -> unitless_pcm (field_types field)))
-    : unitless_pcm (struct_type field_types)
-  =
+      (field_types: (field_id -> Type u#a))
+      (base_pcms: (field: field_id -> unitless_pcm (field_types field)))
+    : unitless_pcm (struct_type field_types) =
   let composable_field (field: field_id) (x y: struct_type field_types) : prop =
     let xf = DepMap.sel x field in
     let yf = DepMap.sel y field in
     (base_pcms field).unitless_p.unitless_composable xf yf
   in
-  let composable : symrel (struct_type field_types) =
+  let composable:symrel (struct_type field_types) =
     fun x y -> forall (field: field_id). composable_field field x y
   in
-  let compose
-    (x: struct_type field_types)
-    (y: struct_type field_types{composable x y})
-      : struct_type field_types
-    =
+  let compose (x: struct_type field_types) (y: struct_type field_types {composable x y})
+      : struct_type field_types =
     DepMap.create (fun field ->
-      let xf = DepMap.sel x field in
-      let yf = DepMap.sel y field in
-      (base_pcms field).unitless_p.unitless_op xf yf
-    )
+          let xf = DepMap.sel x field in
+          let yf = DepMap.sel y field in
+          (base_pcms field).unitless_p.unitless_op xf yf)
   in
-  let pcm' : unitless_pcm' (struct_type field_types) = {
-    unitless_composable = composable;
-    unitless_op = compose;
-  } in
+  let pcm':unitless_pcm' (struct_type field_types) =
+    { unitless_composable = composable; unitless_op = compose }
+  in
   {
     unitless_p = pcm';
-    (* The proofs here should simply follow by generalization for all fields *)
-    unitless_comm = (fun x y -> admit());
-    unitless_assoc = (fun _ _ _ -> admit());
-    unitless_assoc_r = (fun _ _ _ -> admit());
+    unitless_comm
+    =
+    (fun x y ->
+        let xy = pcm'.unitless_op x y in
+        let yx = pcm'.unitless_op y x in
+        let aux (f: field_id) : Lemma (DepMap.sel xy f == DepMap.sel yx f) =
+          (base_pcms f).unitless_comm (DepMap.sel x f) (DepMap.sel y f)
+        in
+        Classical.forall_intro aux;
+        assert (xy `DepMap.equal` yx));
+    unitless_assoc
+    =
+    (fun x y z ->
+        let x_yz = pcm'.unitless_op x (pcm'.unitless_op y z) in
+        let aux (f: field_id)
+            : Lemma
+            (let xf = DepMap.sel x f in
+              let yf = DepMap.sel y f in
+              let zf = DepMap.sel z f in
+              (base_pcms f).unitless_p.unitless_composable xf yf /\
+              (base_pcms f).unitless_p.unitless_composable ((base_pcms f).unitless_p.unitless_op xf
+                    yf)
+                zf /\
+              (base_pcms f).unitless_p.unitless_op xf ((base_pcms f).unitless_p.unitless_op yf zf) ==
+              (base_pcms f).unitless_p.unitless_op ((base_pcms f).unitless_p.unitless_op xf yf) zf)
+        =
+          let xf = DepMap.sel x f in
+          let yf = DepMap.sel y f in
+          let zf = DepMap.sel z f in
+          (base_pcms f).unitless_assoc xf yf zf
+        in
+        Classical.forall_intro aux;
+        let xy_z = pcm'.unitless_op (pcm'.unitless_op x y) z in
+        assert (x_yz `DepMap.equal` xy_z));
+    unitless_assoc_r
+    =
+    (fun x y z ->
+        let xy_z = pcm'.unitless_op (pcm'.unitless_op x y) z in
+        let aux (f: field_id)
+            : Lemma
+            (let xf = DepMap.sel x f in
+              let yf = DepMap.sel y f in
+              let zf = DepMap.sel z f in
+              (base_pcms f).unitless_p.unitless_composable yf zf /\
+              (base_pcms f).unitless_p.unitless_composable xf
+                ((base_pcms f).unitless_p.unitless_op yf zf) /\
+              (base_pcms f).unitless_p.unitless_op ((base_pcms f).unitless_p.unitless_op xf yf) zf ==
+              (base_pcms f).unitless_p.unitless_op xf ((base_pcms f).unitless_p.unitless_op yf zf))
+        =
+          let xf = DepMap.sel x f in
+          let yf = DepMap.sel y f in
+          let zf = DepMap.sel z f in
+          (base_pcms f).unitless_assoc_r xf yf zf
+        in
+        Classical.forall_intro aux;
+        let x_yz = pcm'.unitless_op x (pcm'.unitless_op y z) in
+        assert (x_yz `DepMap.equal` xy_z))
   }
 
 ////////////////////////////////////////////////////////////////////
@@ -216,64 +294,51 @@ let pointwise_struct_pcm
 open Steel.PCM.FractionalPermission
 open Steel.PCM.Unitless.Base
 
-let array_with_frac_perm_on_all_indexes (t: Type u#a) (len: usize) (v: t) : array_struct u#a
-  =
-  ArrayStruct
-    (DArray (DBase (with_perm u#a t)) len)
+let array_with_frac_perm_on_all_indexes (t: Type u#a) (len: usize) (v: t) : array_struct u#a =
+  ArrayStruct (DArray (DBase (with_perm u#a t)) len)
     (pointwise_array_pcm (with_perm t) len frac_perm_pcm)
-    (Seq.init u#a (v_usize len) (fun _ -> { value = v; perm = perm_one} ))
+    (Seq.init u#a (v_usize len) (fun _ -> { value = v; perm = perm_one }))
 
-let immutable_splittable_array (t: Type u#a) (len: usize) (v: t) : array_struct u#a
-  =
-  ArrayStruct
-    (DArray (DBase t) len)
+let immutable_splittable_array (t: Type u#a) (len: usize) (v: t) : array_struct u#a =
+  ArrayStruct (DArray (DBase t) len)
     (pointwise_array_pcm t len immutable_unitless_pcm)
     (Seq.init u#a (v_usize len) (fun _ -> v))
 
 let two_fields_restricted_func
-  (#a: Type u#a)
-  (field1: string)
-  (field2: string{field2 <> field1})
-  (value1 value2 by_default: a)
-  : (field_id ^-> a) =
-  on _ (fun field ->
-    if field = field1 then value1
-    else if field = field2 then value2
-    else by_default
-  )
+      (#a: Type u#a)
+      (field1: string)
+      (field2: string{field2 <> field1})
+      (value1 value2 by_default: a)
+    : (field_id ^-> a) =
+  on _
+    (fun field -> if field = field1 then value1 else if field = field2 then value2 else by_default)
 
 #push-options "--fuel 2 --ifuel 2"
 let two_fields_dep_map
-  (a: field_id -> Type u#a)
-  (field1: string)
-  (field2: string{field2 <> field1})
-  (value1: a field1)
-  (value2: a field2)
-  (by_default: (field:field_id{field <> field1 /\ field <> field2} -> a field))
-  : (DepMap.t field_id a) =
-  DepMap.create #field_id #a (fun field ->
-    if field = field1 then begin admit(); value1 end (* Why can't F* find this ? *)
-    else if field = field2 then begin admit(); value2 end
-    else by_default field
-  )
+      (a: (field_id -> Type u#a))
+      (field1: string)
+      (field2: string{field2 <> field1})
+      (value1: a field1)
+      (value2: a field2)
+      (by_default: (field: field_id{field <> field1 /\ field <> field2} -> a field))
+    : (DepMap.t field_id a) =
+  DepMap.create #field_id
+    #a
+    (fun field ->
+        if field = field1 then value1 else if field = field2 then value2 else by_default field)
 
 
-let point_2d : array_struct =
-  let field_descriptors =
-    two_fields_restricted_func "x" "y" (DBase int) (DBase int) (DBase unit)
-  in
-  let field_types : (field_id -> Type0) = struct_field_type field_descriptors in
-  let field_pcms : (field:field_id -> unitless_pcm (field_types field)) =
+let point_2d:array_struct =
+  let field_descriptors = two_fields_restricted_func "x" "y" (DBase int) (DBase int) (DBase unit) in
+  let field_types:(field_id -> Type0) = struct_field_type field_descriptors in
+  let field_pcms:(field: field_id -> unitless_pcm (field_types field)) =
     fun field ->
-    if field = "x" then
-      exclusive_unitless_pcm
-    else if field = "y" then
-      immutable_unitless_pcm
-    else
-      exclusive_unitless_pcm
+      if field = "x"
+      then exclusive_unitless_pcm
+      else if field = "y" then immutable_unitless_pcm else exclusive_unitless_pcm
   in
   struct_field_type_unroll_lemma field_descriptors;
-  ArrayStruct
-    (DStruct field_descriptors)
+  ArrayStruct (DStruct field_descriptors)
     (pointwise_struct_pcm field_types field_pcms)
     (two_fields_dep_map field_types "x" "y" 0 1 (fun _ -> ()))
+
